Almost done with negshift.

language_formalisation/substitution/substitution_lemmas.v
@@ -103,75 +103,78 @@ revert j; induction h; intros j; simpl; auto.
 Qed.
 
 
-Lemma v_no_var_shift (v:val) j cut:
-  v_no_var v j -> (cut <= j) -> v_no_var (Sub.v_shift v 1 cut) (1+j)
+Lemma v_no_var_shift (v:val) j n cut:
+  v_no_var v j -> (cut <= j) -> v_no_var (Sub.v_shift v n cut) (n+j)
 
-with c_no_var_shift (c:comp) j cut:
-  c_no_var c j -> (cut <= j) -> c_no_var (Sub.c_shift c 1 cut) (1+j)
+with c_no_var_shift (c:comp) j n cut:
+  c_no_var c j -> (cut <= j) -> c_no_var (Sub.c_shift c n cut) (n+j)
   
-with h_no_var_shift (h:hcases) j cut:
-  h_no_var h j -> (cut <= j) -> h_no_var (Sub.h_shift h 1 cut) (1+j).
+with h_no_var_shift (h:hcases) j n cut:
+  h_no_var h j -> (cut <= j) -> h_no_var (Sub.h_shift h n cut) (n+j).
 Proof.
+all: assert (forall j, S(n+j)=n+(S j)) as snj by (intro; omega).
+all: assert (forall j, S(S(n+j))=n+(S(S j))) as ssnj by (intro; omega).
 {
 clear v_no_var_shift.
 revert j. induction v; intros j orig_clean j_le_cut; simpl; simpl in orig_clean;
 try constructor; try inv orig_clean; auto.
 + destruct v as (name, num). destruct (cut <=? num) eqn:cmp; simpl;
   try rewrite leb_iff_conv in cmp; omega.
-+ apply c_no_var_shift. assumption. omega. 
-+ apply c_no_var_shift. assumption. omega.
++ rewrite snj. apply c_no_var_shift. assumption. omega. 
++ rewrite snj. apply c_no_var_shift. assumption. omega.
 }{
 clear c_no_var_shift.
-revert j cut. induction c; intros j cut orig_clean j_le_cut; simpl; simpl in *; 
-try destruct p; try inv orig_clean; try constructor; try constructor; auto;
-try apply IHc || apply IHc1 || apply IHc2; try omega; auto.
+revert j cut. induction c; intros j cut orig_clean j_le_cut; simpl; simpl in *.
+all: try inv orig_clean; try constructor; try constructor; auto.
+all: try rewrite ssnj; try rewrite snj.
+all: try apply IHc || apply IHc1 || apply IHc2; try omega; auto.
 all: inv H0; assumption.
 }{
 clear h_no_var_shift.
 revert j cut. induction h; intros j cut orig_clean j_le_cut; simpl;
 destruct orig_clean; auto. constructor. auto.
-apply c_no_var_shift. assumption. omega.
+rewrite ssnj. apply c_no_var_shift. assumption. omega.
 }
 Qed.
 
 
-Lemma v_no_var_sub (v:val) j v_s :
+Lemma v_no_var_subbed (v:val) j v_s :
   v_no_var v_s j -> v_no_var (Sub.v_sub v (j, v_s)) j
 
-with c_no_var_sub (c:comp) j v_s :
+with c_no_var_subbed (c:comp) j v_s :
   v_no_var v_s j -> c_no_var (Sub.c_sub c (j, v_s)) j
 
-with h_no_var_sub (h:hcases) j v_s :
+with h_no_var_subbed (h:hcases) j v_s :
   v_no_var v_s j -> h_no_var (Sub.h_sub h (j, v_s)) j.
 Proof.
 {
-clear v_no_var_sub.
+clear v_no_var_subbed.
 revert j. induction v; intros j v_s_clean; try constructor.
 all: try (apply IHv; assumption); auto.
 - destruct v as (x, n). simpl.
   induction (n =? j) eqn:fits.
   + assumption.
   + simpl. apply Nat.eqb_neq in fits. omega.
-- apply c_no_var_sub. apply v_no_var_shift. assumption. omega.
-- apply c_no_var_sub. apply v_no_var_shift. assumption. omega.
+- apply c_no_var_subbed. apply v_no_var_shift. assumption. omega.
+- apply c_no_var_subbed. apply v_no_var_shift. assumption. omega.
 }{
-clear c_no_var_sub.
+clear c_no_var_subbed.
 revert j v_s. induction c; intros j v_s v_s_clean; simpl; try constructor;
 try destruct p; simpl; try constructor; auto;
 try apply IHc || apply IHc1 || apply IHc2;
 try (apply v_no_var_shift; assumption || omega).
 all:
 assert (v_no_var (Sub.v_shift v_s 1 0) (1 + j)) by
-  (apply v_no_var_shift; auto || omega);
-apply (v_no_var_shift _ _ 0) in H; try omega.
+  (apply v_no_var_shift; auto || omega).
+all: apply (v_no_var_shift _ _ 1 0) in H; try omega.
 all: rewrite v_shift_shift in H; simpl in H; assumption.
 }{
-clear h_no_var_sub.
+clear h_no_var_subbed.
 revert j v_s. induction h; intros j v_s v_s_clean; simpl; auto.
 constructor. auto.
 assert (v_no_var (Sub.v_shift v_s 1 0) (1+j)).
 { apply v_no_var_shift. auto. omega. }
-apply (v_no_var_shift _ _ 0) in H.
+apply (v_no_var_shift _ _ 1 0) in H.
 rewrite (v_shift_shift _ _ _) in H. auto. omega.
 }
 Qed.
@@ -294,7 +297,7 @@ all : try reflexivity || apply IHv || apply IHv1 || apply IHv2.
 all : try apply c_negshift_shift || apply h_negshift_shift; assumption.
 }{
 clear c_negshift_shift h_negshift_shift.
-revert cut. induction c; intros cut m_le_n; try destruct p; simpl; f_equal;
+revert cut. induction c; intros cut m_le_n; simpl; f_equal;
 try apply v_negshift_shift || apply IHc || apply IHc1 || apply IHc2; assumption.
 }{
 clear h_negshift_shift v_negshift_shift.
@@ -303,6 +306,60 @@ reflexivity. apply IHh. assumption. apply c_negshift_shift. assumption.
 }
 Qed.
 
+Lemma v_shift_negshift_1j v n i j :
+v_no_var v j -> i <= j ->
+  Sub.v_shift (Sub.v_negshift v 1 j) n i 
+= Sub.v_negshift (Sub.v_shift v n i) 1 (n+j) 
+with c_shift_negshift_1j c n i j :
+c_no_var c j -> i <= j ->
+  Sub.c_shift (Sub.c_negshift c 1 j) n i 
+= Sub.c_negshift (Sub.c_shift c n i) 1 (n+j) 
+with h_shift_negshift_1j h n i j :
+h_no_var h j -> i <= j ->
+  Sub.h_shift (Sub.h_negshift h 1 j) n i 
+= Sub.h_negshift (Sub.h_shift h n i) 1 (n+j).
+Proof.
+{
+clear v_shift_negshift_1j.
+revert j; induction v; intros j novar cmpij; simpl.
+{ 
+destruct v as (x, d). simpl.
+destruct (j<=?d) eqn:jd.
++ apply leb_complete in jd. assert (i<=?d=true) by (apply leb_correct; omega).
+  rewrite H. simpl. assert (n+j<=?n+d=true).
+  { apply leb_correct; omega. }
+  rewrite H0. assert (i<=?d-1=true).
+  { apply leb_correct. simpl in novar. omega. }
+  rewrite H1. do 2 f_equal. simpl in novar. omega.
++ apply leb_complete_conv in jd. simpl.
+  destruct (i<=?d) eqn:id; simpl.
+  - assert (n+j<=?n+d=false).
+    { apply leb_correct_conv; omega. }
+    rewrite H. reflexivity.
+  - assert (n+j<=?d=false).
+    { apply leb_correct_conv; omega. }
+    rewrite H. reflexivity.
+}
+all : f_equal; try reflexivity || apply IHv || apply IHv1 || apply IHv2.
+all : simpl in novar; try destruct novar; auto.
+all : assert (S(n+j)=n+(S j)) as snj by omega; rewrite snj.
+all : apply c_shift_negshift_1j; omega || auto.
+}{
+clear h_shift_negshift_1j.
+revert j. destruct c; intros j novar cmpij; simpl in *; f_equal.
+all : assert (S(S(n+j))=n+(S (S j))) as ssnj by omega; try rewrite ssnj.
+all : assert (S(n+j)=n+(S j)) as snj by omega; try rewrite snj.
+all: apply v_shift_negshift_1j || apply c_shift_negshift_1j.
+all: omega || (try destruct novar; auto).
+all: destruct H0; auto.
+}{
+clear h_shift_negshift_1j v_shift_negshift_1j.
+revert j. induction h; intros j novar cmpij; simpl; f_equal. auto.
++ apply IHh. inv novar. assumption. assumption.
++ assert (S(S(n+j))=n+(S (S j))) as ssnj by omega; try rewrite ssnj.
+  apply c_shift_negshift_1j. inv novar. auto. omega.
+}
+Qed.
 
 
 Lemma v_shift_0 cut v : Sub.v_shift v 0 cut = v
@@ -407,7 +464,7 @@ all: rewrite c_shift_sub; clear c_shift_sub; try omega.
 all: do 3 f_equal; rewrite (v_shift_comm_aux 1 j); f_equal; try omega.
 all: rewrite (v_shift_comm_aux 1 i); f_equal; omega.
 }{
-induction c; unfold c_sub; simpl; f_equal;
+destruct c; unfold c_sub; simpl; f_equal;
 try apply v_shift_sub; try assumption.
 all: clear v_shift_sub h_shift_sub; unfold c_sub in c_shift_sub.
 + rewrite <-(v_shift_shift 1), (v_shift_comm_aux 1 j).
@@ -437,10 +494,14 @@ all: clear v_shift_sub h_shift_sub; unfold c_sub in c_shift_sub.
   do 3 f_equal. rewrite (v_shift_comm_aux 1 j). f_equal.
   rewrite (v_shift_comm_aux 1 i). f_equal. all: omega.
 + rewrite v_shift_comm_aux. rewrite c_shift_sub. clear c_shift_sub.
+  do 2 f_equal. rewrite (v_shift_comm_aux). reflexivity. all: omega.
++ rewrite v_shift_comm_aux. rewrite c_shift_sub. clear c_shift_sub.
   do 3 f_equal. rewrite (v_shift_comm_aux 1 j). f_equal.
   rewrite (v_shift_comm_aux 1 i). f_equal. all: omega.
++ rewrite v_shift_comm_aux. rewrite c_shift_sub. clear c_shift_sub.
+  do 2 f_equal. rewrite (v_shift_comm_aux). reflexivity. all: omega.
 }{
-induction h; unfold h_sub; simpl. auto. f_equal.
+destruct h; unfold h_sub; simpl. auto. f_equal.
 + apply h_shift_sub. assumption.
 + clear v_shift_sub h_shift_sub.
   unfold c_sub in c_shift_sub.
@@ -456,133 +517,125 @@ Qed.
 
 
 Lemma v_negshift_sub v v' i j (safe: j <= i): 
-  v_no_var v i -> v_no_var v' i ->
+  v_no_var v (1+i) -> v_no_var v' (i) ->
   Sub.v_negshift (v_sub v v' j) 1 i = 
-  (v_sub (Sub.v_negshift v 1 (i+1)) (Sub.v_negshift v' 1 i) j)
+  (v_sub (Sub.v_negshift v 1 (1+i)) (Sub.v_negshift v' 1 i) j)
 with c_negshift_sub c v' i j (safe: j <= i): 
-  c_no_var c i -> v_no_var v' i ->
+  c_no_var c (1+i) -> v_no_var v' (i) ->
   Sub.c_negshift (c_sub c v' j) 1 i = 
-  (c_sub (Sub.c_negshift c 1 (i+1)) (Sub.v_negshift v' 1 i) j)
+  (c_sub (Sub.c_negshift c 1 (1+i)) (Sub.v_negshift v' 1 i) j)
 with h_negshift_sub h v' i j (safe: j <= i): 
-  h_no_var h i -> v_no_var v' i ->
+  h_no_var h (1+i) -> v_no_var v' (i) ->
   Sub.h_negshift (h_sub h v' j) 1 i = 
-  (h_sub (Sub.h_negshift h 1 (i+1)) (Sub.v_negshift v' 1 i) j).
+  (h_sub (Sub.h_negshift h 1 (1+i)) (Sub.v_negshift v' 1 i) j).
 Proof.
 {
 intros nov nov'. destruct v; unfold v_sub; simpl.
 {
-clear v_negshift_sub c_negshift_sub h_negshift_sub.
-destruct v as (x, n). 
-destruct (n=?j) eqn:nj.
-apply Nat.eqb_eq in nj. subst.
-
-(* HERE WE ARE *)
-
-
-+ destruct (i+1=?j) eqn:eqij.
-  - apply Nat.eqb_eq in eqij. subst.
-    assert (1+j<=?j=false) by (apply leb_correct_conv; omega).
-    simpl in H. rewrite H. simpl.
-    assert (j=?j=true) by (apply Nat.eqb_eq; reflexivity).
-    rewrite H0. simpl. 
-    rewrite v_negshift_shift. rewrite v_negshift_shift.
-    rewrite v_shift_shift. rewrite v_shift_shift. f_equal.
-    omega. omega.
-  - assert (1+i<=?i=false) by (apply leb_correct_conv; omega).
-    simpl in H. rewrite H. simpl.
-    assert (j<=?i=true) by (apply leb_correct;omega).
-    rewrite H0. rewrite eqij. simpl. rewrite H0.
-    assert (i<=?i-1=false).
-    { apply leb_correct_conv. apply Nat.eqb_neq in eqij. 
-      apply leb_complete in H0. omega. }
-    rewrite H1. reflexivity.
-+ destruct (n=?j) eqn:nj.
-  ++apply Nat.eqb_eq in nj. subst.
-    assert (1+i<=?j=false) by (apply leb_correct_conv; omega).
-    simpl in H. rewrite H.
-    simpl. assert (j=?j=true) by (apply Nat.eqb_eq; omega).
-    rewrite H0. rewrite v_negshift_shift. rewrite v_negshift_shift. simpl.
-    rewrite v_shift_0. rewrite v_shift_0.
+  clear v_negshift_sub c_negshift_sub h_negshift_sub.
+  destruct v as (x, n).
+  destruct (n=?j) eqn:nj.
+  apply Nat.eqb_eq in nj. subst.
+  destruct (1+i <=? j) eqn:cmpij.
+  3 : destruct (1+i <=? n) eqn:Sin.
+  all: simpl.
+  + apply leb_complete in cmpij.
+    assert (j=S i) by omega. subst. omega.
+  + simpl in cmpij. rewrite cmpij. simpl.
+    assert (j=?j=true) by (apply Nat.eqb_eq; omega).
+    rewrite H, v_negshift_shift, v_shift_0, v_negshift_shift, v_shift_0.
     reflexivity. omega. omega.
-  ++destruct (i<=?n) eqn:iln; simpl.
-    - destruct (j<=?n) eqn:jln; simpl.
-      * apply leb_complete in jln. apply leb_complete in iln.
-        assert (i<=?n-1=true).
-        { apply leb_correct. apply Nat.eqb_neq in ni. omega. }
-        rewrite H. simpl. assert (1+i<=?n=true).
-        { apply leb_correct. apply leb_complete in H.
-          apply Nat.eqb_neq in ni. omega. }
-        simpl in H0. rewrite H0. simpl. 
-        assert (1+n=?j=false).
-        { apply Nat.eqb_neq. omega. }
-        simpl in H1. rewrite H1. simpl. assert (j<=? S n=true).
-        { apply leb_correct. omega. }
-        rewrite H2. simpl.
-        f_equal. f_equal. assert (n>0) by (apply Nat.eqb_neq in ni; omega).
-        omega.
-      * apply leb_complete in iln. apply leb_complete_conv in jln. omega.
-    - apply leb_complete_conv in iln.
-      assert (1+i<=?n=false) by (apply leb_correct_conv; omega).
-      simpl in H. rewrite H. simpl. rewrite nj. simpl.
-      destruct (j<=?n) eqn:jln.
-      * simpl. assert (i<=?n-1=false).
-        { apply leb_correct_conv. omega. }
-        rewrite H0. reflexivity.
-      * simpl. assert (i<=?n=false) by (apply leb_correct_conv; omega).
-        rewrite H0. reflexivity.
-}     
-all: f_equal; auto.
-3: apply h_shift_sub; auto.
-all: clear v_shift_sub h_shift_sub; unfold c_sub in c_shift_sub.
-all: rewrite v_shift_comm_aux; try omega.
-all: rewrite c_shift_sub; clear c_shift_sub; try omega.
-all: do 3 f_equal; rewrite (v_shift_comm_aux 1 j); f_equal; try omega.
-all: rewrite (v_shift_comm_aux 1 i); f_equal; omega.
+  + apply leb_complete in Sin as sin. simpl in Sin.
+    rewrite Sin. apply Nat.eqb_neq in nj.
+    assert (j<=?n=true) by (apply leb_correct; omega). simpl in H.
+    rewrite H. simpl. assert (i<=?n-1=true) by (apply leb_correct; omega).
+    rewrite H0. assert (n-1=?j=false).
+    { apply Nat.eqb_neq. simpl in nov. omega. }
+    rewrite H1. simpl. assert (j<=?n-1=true).
+    { apply leb_correct. omega. }
+    rewrite H2. reflexivity.
+  + apply leb_complete_conv in Sin as sin. simpl in Sin. rewrite Sin. simpl.  
+    rewrite nj. apply Nat.eqb_neq in nj. simpl.
+    destruct (j<=?n) eqn:jln.
+    - simpl. assert (i<=?n-1=false).
+      { apply leb_correct_conv. omega. }
+      rewrite H. reflexivity.
+    - simpl. assert (i<=?n=false).
+      { apply leb_correct_conv. apply leb_complete_conv in jln. omega. }
+      rewrite H. reflexivity. 
+}
+all: f_equal; simpl in nov.
+all: try apply v_negshift_sub; try omega || auto.
+5: apply h_negshift_sub; auto; destruct nov; auto.
++ destruct nov. auto.
++ destruct nov. auto.
++ unfold c_sub in c_negshift_sub. rewrite v_shift_comm_aux.
+  rewrite (c_negshift_sub c _ (S i) (S j)). clear c_negshift_sub.
+  do 3 f_equal. rewrite v_shift_comm_aux. f_equal.
+  rewrite v_shift_negshift_1j. all: omega || auto.
+  apply v_no_var_shift. auto. omega.
++ unfold c_sub in c_negshift_sub. rewrite v_shift_comm_aux. destruct nov.
+  rewrite (c_negshift_sub c _ (S i) (S j)). clear c_negshift_sub.
+  do 3 f_equal. rewrite v_shift_comm_aux. f_equal.
+  rewrite v_shift_negshift_1j. all: omega || auto.
+  apply v_no_var_shift. auto. omega.
 }{
-induction c; unfold c_sub; simpl; f_equal;
-try apply v_shift_sub; try assumption.
-all: clear v_shift_sub h_shift_sub; unfold c_sub in c_shift_sub.
+induction c; intros nov nov'; unfold c_sub; simpl in nov |-*; f_equal;
+try apply v_negshift_sub; try assumption.
+all: clear v_negshift_sub h_negshift_sub.
+all: try (destruct nov; assumption).
+all: unfold c_sub in c_negshift_sub; inv nov.
 + rewrite <-(v_shift_shift 1), (v_shift_comm_aux 1 j).
-  rewrite (v_shift_comm_aux 1 (1+j)), c_shift_sub. clear c_shift_sub. simpl.
-  do 2 f_equal. all: try omega.
-  rewrite <-(v_shift_shift 1 1 0), (v_shift_comm_aux 1 j).
+  rewrite (v_shift_comm_aux 1 (1+j)), c_negshift_sub. clear c_negshift_sub. simpl. do 3 f_equal. rewrite <-(v_shift_shift 1 1 0), (v_shift_comm_aux 1 j).
   rewrite (v_shift_comm_aux 1 (1+j)). f_equal. 
-  rewrite (v_shift_comm_aux 1 i), (v_shift_comm_aux 1 (1+i)). 
-  do 2 f_equal. all: omega.
-+ rewrite v_shift_comm_aux. rewrite c_shift_sub. clear c_shift_sub.
-  do 3 f_equal. rewrite (v_shift_comm_aux 1 j). f_equal.
-  rewrite (v_shift_comm_aux 1 i). f_equal. all: omega.
-+ rewrite v_shift_comm_aux. rewrite c_shift_sub. clear c_shift_sub.
-  do 3 f_equal. rewrite (v_shift_comm_aux 1 j). f_equal.
-  rewrite (v_shift_comm_aux 1 i). f_equal. all: omega.
-+ rewrite v_shift_comm_aux. rewrite c_shift_sub. clear c_shift_sub.
-  do 3 f_equal. rewrite (v_shift_comm_aux 1 j). f_equal.
-  rewrite (v_shift_comm_aux 1 i). f_equal. all: omega.
+  rewrite v_shift_shift, v_shift_shift, v_shift_negshift_1j. reflexivity. 
+  all: omega || auto. apply v_no_var_shift. apply v_no_var_shift.
+  auto. omega. omega.
++ rewrite v_shift_comm_aux. inv H0.
+  rewrite (c_negshift_sub _ _ (S i) (S j)). clear c_negshift_sub.
+  do 3 f_equal. rewrite v_shift_comm_aux. f_equal.
+  rewrite v_shift_negshift_1j. all: omega || auto.
+  apply v_no_var_shift. auto. omega.
++ rewrite v_shift_comm_aux. inv H0.
+  rewrite (c_negshift_sub _ _ (S i) (S j)). clear c_negshift_sub.
+  do 3 f_equal. rewrite v_shift_comm_aux. f_equal.
+  rewrite v_shift_negshift_1j. all: omega || auto.
+  apply v_no_var_shift. auto. omega.
++ rewrite v_shift_comm_aux.
+  rewrite (c_negshift_sub _ _ (S i) (S j)). clear c_negshift_sub.
+  do 3 f_equal. rewrite v_shift_comm_aux. f_equal.
+  rewrite v_shift_negshift_1j. all: omega || auto.
+  apply v_no_var_shift. auto. omega.
 + rewrite <-(v_shift_shift 1), (v_shift_comm_aux 1 j).
-  rewrite (v_shift_comm_aux 1 (1+j)), c_shift_sub. clear c_shift_sub. simpl.
-  do 2 f_equal. all: try omega.
-  rewrite <-(v_shift_shift 1 1 0), (v_shift_comm_aux 1 j).
+  rewrite (v_shift_comm_aux 1 (1+j)), c_negshift_sub. clear c_negshift_sub. simpl. do 3 f_equal. rewrite <-(v_shift_shift 1 1 0), (v_shift_comm_aux 1 j).
   rewrite (v_shift_comm_aux 1 (1+j)). f_equal. 
-  rewrite (v_shift_comm_aux 1 i), (v_shift_comm_aux 1 (1+i)). 
-  do 2 f_equal. all: omega.
-+ rewrite v_shift_comm_aux. rewrite c_shift_sub. clear c_shift_sub.
-  do 3 f_equal. rewrite (v_shift_comm_aux 1 j). f_equal.
-  rewrite (v_shift_comm_aux 1 i). f_equal. all: omega.
-+ rewrite v_shift_comm_aux. rewrite c_shift_sub. clear c_shift_sub.
-  do 3 f_equal. rewrite (v_shift_comm_aux 1 j). f_equal.
-  rewrite (v_shift_comm_aux 1 i). f_equal. all: omega.
+  rewrite v_shift_shift, v_shift_shift, v_shift_negshift_1j. reflexivity. 
+  all: omega || auto. apply v_no_var_shift. apply v_no_var_shift.
+  auto. omega. omega.
++ rewrite v_shift_comm_aux.
+  rewrite (c_negshift_sub _ _ (S i) (S j)). clear c_negshift_sub.
+  do 3 f_equal. rewrite v_shift_comm_aux. f_equal.
+  rewrite v_shift_negshift_1j. all: omega || auto.
+  apply v_no_var_shift. auto. omega.
++ rewrite c_negshift_sub. clear c_negshift_sub.
+  do 3 f_equal. all: omega || auto.
++ rewrite v_shift_comm_aux.
+  rewrite (c_negshift_sub _ _ (S i) (S j)). clear c_negshift_sub.
+  do 3 f_equal. rewrite v_shift_comm_aux. f_equal.
+  rewrite v_shift_negshift_1j. all: omega || auto.
+  apply v_no_var_shift. auto. omega.
++ rewrite c_negshift_sub. clear c_negshift_sub.
+  do 3 f_equal. all: omega || auto.
 }{
-induction h; unfold h_sub; simpl. auto. f_equal.
-+ apply h_shift_sub. assumption.
-+ clear v_shift_sub h_shift_sub.
-  unfold c_sub in c_shift_sub.
-  rewrite <-(v_shift_shift 1), (v_shift_comm_aux 1 j).
-  rewrite (v_shift_comm_aux 1 (1+j)), c_shift_sub. clear c_shift_sub. simpl.
-  do 2 f_equal. all: try omega.
-  rewrite <-(v_shift_shift 1 1 0), (v_shift_comm_aux 1 j).
+destruct h; unfold h_sub; intros nov nov'; simpl. auto. inv nov. f_equal.
++ apply h_negshift_sub; auto.
++ unfold c_sub in c_negshift_sub. clear v_negshift_sub h_negshift_sub.
+  rewrite <-(v_shift_shift 1), (v_shift_comm_aux 1 j). simpl.
+  rewrite (v_shift_comm_aux 1 (1+j)), c_negshift_sub. clear c_negshift_sub. simpl. do 3 f_equal. rewrite <-(v_shift_shift 1 1 0), (v_shift_comm_aux 1 j).
   rewrite (v_shift_comm_aux 1 (1+j)). f_equal. 
-  rewrite (v_shift_comm_aux 1 i), (v_shift_comm_aux 1 (1+i)). 
-  do 2 f_equal. all: omega.
+  rewrite v_shift_shift, v_shift_shift, v_shift_negshift_1j. reflexivity. 
+  all: omega || auto. apply v_no_var_shift. apply v_no_var_shift.
+  auto. omega. omega.
 }
 Qed.
 
@@ -661,4 +714,90 @@ all: destruct H0; auto.
 intros under. destruct h; simpl; simpl in under.
 all: try (destruct under; f_equal; auto) || (f_equal; auto).
 }
+Qed.
+
+
+Fixpoint v_under_var_sub v v' i j {struct v}:
+  v_under_var v i -> v_under_var v' i -> v_under_var (v_sub v v' j) i
+with c_under_var_sub c v' i j {struct c}:
+  c_under_var c i -> v_under_var v' i -> c_under_var (c_sub c v' j) i
+with h_under_var_sub h v' i j {struct h}:
+  h_under_var h i -> v_under_var v' i -> h_under_var (h_sub h v' j) i.
+Proof.
+all: revert i j.
++ intros. destruct v.
+  { destruct v as (x,d). unfold v_sub. simpl. simpl in H.
+    destruct (d=?j).
+    + rewrite v_negshift_shift, v_shift_0. auto. omega.
+    + simpl. destruct (j<=?d); simpl; omega.
+  }
+  all: simpl in *; auto.
+  - apply v_under_var_sub; auto.
+  - apply v_under_var_sub; auto.
+  - constructor; inv H; apply v_under_var_sub; auto.
+  - rewrite v_shift_comm_aux. apply c_under_var_sub. auto.
+    apply v_under_var_shift. auto. omega. omega.
+  - constructor; inv H.
+    * rewrite v_shift_comm_aux. apply c_under_var_sub. auto.
+      apply v_under_var_shift. auto. omega. omega.
+    * apply h_under_var_sub; auto.
++ intros. induction c; simpl in *; auto.
+  all: try constructor; try inv H; auto.
+  all: try apply v_under_var_sub; eauto.
+  2: constructor; inv H2.
+  all: rewrite v_shift_comm_aux; try apply c_under_var_sub; omega || auto.
+  all: try apply v_under_var_shift; omega || auto.
+  all: assert (S(S i) = 2+i) by omega; rewrite H; apply v_under_var_shift.
+  all: omega || auto.
++ intros. induction h; simpl in *; auto.
+  constructor; inv H; auto.
+  rewrite v_shift_comm_aux; try apply c_under_var_sub; omega || auto.
+  assert (S(S i) = 2+i) by omega; rewrite H; apply v_under_var_shift.
+  auto. omega.
+Qed.
+
+
+Fixpoint v_no_var_sub v v' i j {struct v}:
+  v_no_var v (1+i) -> v_no_var v' i -> j<i ->
+  v_no_var (v_sub v v' j) i
+with c_no_var_sub c v' i j {struct c}:
+  c_no_var c (1+i) -> v_no_var v' i -> j<i ->
+  c_no_var (c_sub c v' j) i
+with h_no_var_sub h v' i j {struct h}:
+  h_no_var h (1+i) -> v_no_var v' i -> j<i ->
+  h_no_var (h_sub h v' j) i.
+Proof.
+all: revert i j.
++ intros. destruct v.
+  { 
+    destruct v as (x,d). unfold v_sub. simpl. simpl in H.
+    destruct (d=?j) eqn:dj.
+    + rewrite v_negshift_shift, v_shift_0. auto. omega.
+    + simpl. destruct (j<=?d) eqn:jld; simpl; apply Nat.eqb_neq in dj.
+      - apply leb_complete in jld. omega.
+      - apply leb_complete_conv in jld. omega.
+  }
+  all: simpl in *; auto.
+  - apply v_no_var_sub; auto.
+  - apply v_no_var_sub; auto.
+  - constructor; inv H; apply v_no_var_sub; auto.
+  - rewrite v_shift_comm_aux. apply c_no_var_sub. auto.
+    apply v_no_var_shift. auto. all: omega.
+  - constructor; inv H.
+    * rewrite v_shift_comm_aux. apply c_no_var_sub. auto.
+      apply v_no_var_shift. auto. all: omega.
+    * apply h_no_var_sub; auto.
++ intros. induction c; simpl in *; auto.
+  all: try constructor; try inv H; auto.
+  all: try apply v_no_var_sub; eauto.
+  2: constructor; inv H3.
+  all: rewrite v_shift_comm_aux; try apply c_no_var_sub; omega || auto.
+  all: try apply v_no_var_shift; omega || auto.
+  all: assert (S(S i) = 2+i) by omega; rewrite H; apply v_no_var_shift.
+  all: omega || auto.
++ intros. induction h; simpl in *; auto.
+  constructor; inv H; auto.
+  rewrite v_shift_comm_aux; try apply c_no_var_sub; omega || auto.
+  assert (S(S i) = 2+i) by omega; rewrite H; apply v_no_var_shift.
+  auto. omega.
 Qed.
